m

DynamoDbEncryptionMiddlewareInternal/src/TransactWriteItemsTransform.dfy
@@ -12,16 +12,8 @@ module TransactWriteItemsTransform {
   import EncTypes = AwsCryptographyDynamoDbItemEncryptorTypes
   import Seq
 
-  predicate method {:opaque} IsValid(item : DDB.TransactWriteItem) {
+  predicate method {:opaque} IsValidDDBTransactWrite(item : DDB.TransactWriteItem) {
     item.Put.Some? || item.Update.Some? || item.Delete.Some? || item.ConditionCheck.Some?
-  }
-
-  predicate {:opaque} IsValidTransform(oldItem : DDB.TransactWriteItem, newItem : DDB.TransactWriteItem, config : map<string, ValidTableConfig>) {
-    && oldItem.ConditionCheck == newItem.ConditionCheck
-    && oldItem.Delete == newItem.Delete
-    && oldItem.Update == newItem.Update
-    && (oldItem.Put.None? ==> oldItem.Put == newItem.Put)
-    && (oldItem.Put.Some? && oldItem.Put.value.TableName !in config ==> oldItem.Put == newItem.Put)
   }
 
   method {:vcs_split_on_every_assert} Input(config: Config, input: TransactWriteItemsInputTransformInput)
@@ -36,28 +28,9 @@ module TransactWriteItemsTransform {
     //# To protect against a possible fifth field being added to the TransactWriteItem structure in the future,
     //# the client MUST fail if none of the `Update`, `ConditionCheck`, `Delete` and `Put` fields are set.
     ensures output.Success? ==>
-      forall item <- input.sdkInput.TransactItems :: IsValid(item)
-
-    //= specification/dynamodb-encryption-client/ddb-sdk-integration.md#encrypt-before-transactwriteitems
-    //# Any actions other than `Put, MUST be unchanged.
-
-    //= specification/dynamodb-encryption-client/ddb-sdk-integration.md#encrypt-before-transactwriteitems
-    //# Any `Put` actions  with a `TableName` that does not refer to an [encrypted-table](#encrypted-table),
-    //# MUST be unchanged.
-    // The below has inexplicably become too difficult for Dafny
-    /*
-    ensures output.Success? ==>
-      && var result := output.value.transformedInput.TransactItems;
-      && forall i : nat | 0 <= i < |result| ::
-        && var item := input.sdkInput.TransactItems[i];
-        && item.ConditionCheck == result[i].ConditionCheck
-        && item.Delete == result[i].Delete
-        && item.Update == result[i].Update
-        && (item.Put.None? ==> item.Put == result[i].Put)
-        && (item.Put.Some? && item.Put.value.TableName !in config.tableEncryptionConfigs ==> item.Put == result[i].Put)
-        */
+      forall item <- input.sdkInput.TransactItems :: IsValidDDBTransactWrite(item)
   {
-    :- Need(forall item <- input.sdkInput.TransactItems :: IsValid(item), E("Each item in TransactWriteItems must specify at least one operation"));
+    :- Need(forall item <- input.sdkInput.TransactItems :: IsValidDDBTransactWrite(item), E("Each item in TransactWriteItems must specify at least one supported operation"));
     var result : seq<DDB.TransactWriteItem> := [];
     for x := 0 to |input.sdkInput.TransactItems|
       invariant |result| == x
